Checkpoint initiator verification.

nsl.v
@@ -1,8 +1,8 @@
 From mathcomp Require Import ssreflect.
 From stdpp Require Import gmap.
-From iris.algebra Require Import agree auth gset gmap excl dra sts.
+From iris.algebra Require Import agree auth csum gset gmap excl dra sts.
 From iris.heap_lang Require Import notation proofmode.
-From crypto Require Import term crypto1 primitives.
+From crypto Require Import lib term crypto1 primitives.
 
 Set Implicit Arguments.
 Unset Strict Implicit.
@@ -21,6 +21,24 @@ Inductive session :=
 Inductive turn := Init | Resp.
 
 Canonical turnO := leibnizO turn.
+
+Implicit Types tr : turn.
+
+Lemma turn_equivI tr1 tr2 :
+  tr1 ≡ tr2 ⊣⊢@{iPropI Σ}
+  match tr1, tr2 with
+  | Init, Init | Resp, Resp => True
+  | _, _ => False
+  end.
+Proof.
+by case: tr1 tr2=> [] []; iSplit=> //.
+Qed.
+
+Definition csum_of_turn tr : csum unit unit :=
+  match tr with
+  | Init => Cinl ()
+  | Resp => Cinr ()
+  end.
 
 Implicit Types (s : session) (t : term).
 
@@ -41,49 +59,168 @@ Canonical session_sts : stsT := Sts session_step session_token.
 
 Class nslG := {
   in_nsl_sessG :> inG Σ (gmapUR term (stsR session_sts));
-  in_nsl_keysG :> inG Σ (authR (gmapUR loc (agreeR turnO)));
+  in_nsl_keysG :> inG Σ (authR (gmapUR loc (csumR unitR unitR)));
   nsl_sess_name : gname;
   nsl_keys_name : gname;
 }.
 
 Context `{!nslG}.
 
+Definition initiator_view t s :=
+  own nsl_sess_name {[t := sts_frag_up s {[Init]}]}.
+
+Definition responder_view t s :=
+  own nsl_sess_name {[t := sts_frag_up s {[Resp]}]}.
+
+Definition session_bound t s :=
+  own nsl_sess_name {[t := sts_frag_up s ∅]}.
+
 Definition initiator_key l : iProp Σ :=
-  own nsl_keys_name (◯ {[l := to_agree Init]}).
+  own nsl_keys_name (◯ {[l := csum_of_turn Init]}).
+
+Global Instance initiator_key_persistent l : Persistent (initiator_key l).
+Proof. apply _. Qed.
 
 Definition responder_key l : iProp Σ :=
-  own nsl_keys_name (◯ {[l := to_agree Resp]}).
+  own nsl_keys_name (◯ {[l := csum_of_turn Resp]}).
+
+Global Instance responder_key_persistent l : Persistent (responder_key l).
+Proof. apply _. Qed.
 
 Definition initiator_pred lA t : iProp Σ :=
   match t with
-  | TPair (TNonce nA) (TPair (TNonce nB) (TKey KAEnc lB)) =>
-    nonceT {[lA; lB]} nA ∗ nonceT {[lA; lB]} nB ∗ responder_key lB
+  | TPair (TNonce nA) (TPair (TNonce nB) (TPair (TKey KAEnc lB) _)) =>
+    nonceT {[lA; lB]} nA ∗
+    nonceT {[lA; lB]} nB ∗
+    responder_key lB ∗
+    session_bound (TNonce nA) (SAnswered (TNonce nB) false)
   | _ => False
   end.
+
+Global Instance initiator_pred_proper : NonExpansive2 initiator_pred.
+Proof. solve_contractive. Qed.
 
 Definition responder_pred lB t : iProp Σ :=
   match t with
   | TPair (TNonce nA) (TKey KAEnc lA) =>
     nonceT {[lA; lB]} nA ∗ initiator_key lA
   | TNonce nB =>
-    ∃ lA, nonceT {[lA; lB]} nB ∗ initiator_key lA
+    ∃ nA lA, nonceT {[lA; lB]} nB ∗
+             initiator_key lA ∗
+             session_bound nA (SAnswered (TNonce nB) true)
   | _ => False
   end.
 
-Definition initiator (send recv skA pkA pkB nA : val) : val := λ: <>,
+Global Instance responder_pred_proper : NonExpansive2 responder_pred.
+Proof. solve_contractive. Qed.
+
+Ltac solve_agent_pred :=
+  repeat match goal with
+  | |- ∀ (t : term), _ => case; try by move=> *; apply _
+  | |- ∀ (kt : key_type), _ => case; try by move=> *; apply _
+  | |- ∀ (x : _), _ => move=> ?
+  end.
+
+Global Instance initiator_pred_persistent lA t :
+  Persistent (initiator_pred lA t).
+Proof. move: t; solve_agent_pred. Qed.
+
+Global Instance responder_pred_persistent lB t :
+  Persistent (responder_pred lB t).
+Proof. move: t; solve_agent_pred. Qed.
+
+Definition agent_pred (x : turn) l :=
+  match x with
+  | Init => OfeMor (initiator_pred l)
+  | Resp => OfeMor (responder_pred l)
+  end.
+
+Global Instance agent_pred_persistent x l t :
+  Persistent (agent_pred x l t).
+Proof. by case: x; apply _. Qed.
+
+Implicit Types SM : gmap term session.
+Implicit Types KM : gmap loc turn.
+
+Definition nsl_keys_inv : iProp Σ :=
+  ∃ KM, own nsl_keys_name (● (csum_of_turn <$> KM : gmap _ _)) ∗
+        [∗ map] l ↦ x ∈ KM, akeyT RPub ∅ (agent_pred x l) l.
+
+Definition nsl_sess_inv : iProp Σ :=
+  ∃ SM, own nsl_sess_name ((λ s, sts_auth s ∅) <$> SM : gmap _ _).
+
+Lemma nsl_sess_inv_timeless : Timeless nsl_sess_inv.
+Proof. apply _. Qed.
+
+Lemma initiator_move nA nB :
+  nsl_sess_inv -∗
+  initiator_view nA SNew -∗
+  session_bound nA (SAnswered nB false) ==∗
+  nsl_sess_inv ∗
+  initiator_view nA (SAnswered nB true) ∗
+  session_bound nA (SAnswered nB true).
+Proof. Admitted.
+
+Lemma initiator_key_akey lA :
+  nsl_keys_inv -∗
+  initiator_key lA -∗
+  akeyT RPub ∅ (agent_pred Init lA) lA.
+Proof.
+iDestruct 1 as (KM) "[Hown Hkeys]"; iIntros "HlA".
+iPoseProof (own_valid_2 with "Hown HlA") as "#Hvalid".
+rewrite auth_both_validI.
+iDestruct "Hvalid" as "(_ & Hvalid & _)".
+iDestruct "Hvalid" as (KM') "HKM".
+rewrite gmap_equivI; iSpecialize ("HKM" $! lA).
+rewrite lookup_fmap lookup_op lookup_singleton option_equivI.
+move KM_lA: (KM !! lA)=> o; case: o KM_lA=> [tr|] KM_lA; last first.
+  by rewrite /=; move: (KM' !! lA); case.
+rewrite /=; case: tr KM_lA=> KM_lA; last first.
+  move: (KM' !! lA); case=> [ag|] /=; last first.
+    by rewrite csum_equivI.
+  by case: ag=> *; rewrite csum_equivI.
+iClear "HKM".
+by rewrite big_sepM_delete //; iDestruct "Hkeys" as "[??]".
+Qed.
+
+Lemma responder_key_akey lB :
+  nsl_keys_inv -∗
+  responder_key lB -∗
+  akeyT RPub ∅ (agent_pred Resp lB) lB.
+Proof.
+iDestruct 1 as (KM) "[Hown Hkeys]"; iIntros "HlA".
+iPoseProof (own_valid_2 with "Hown HlA") as "#Hvalid".
+rewrite auth_both_validI.
+iDestruct "Hvalid" as "(_ & Hvalid & _)".
+iDestruct "Hvalid" as (KM') "HKM".
+rewrite gmap_equivI; iSpecialize ("HKM" $! lB).
+rewrite lookup_fmap lookup_op lookup_singleton option_equivI.
+move KM_lB: (KM !! lB)=> o; case: o KM_lB=> [tr|] KM_lB; last first.
+  by rewrite /=; move: (KM' !! lB); case.
+rewrite /=; case: tr KM_lB=> KM_lB.
+  move: (KM' !! lB); case=> [ag|] /=; last first.
+    by rewrite csum_equivI.
+  by case: ag=> *; rewrite csum_equivI.
+iClear "HKM".
+by rewrite big_sepM_delete //; iDestruct "Hkeys" as "[??]".
+Qed.
+
+Variable send recv : val.
+
+Definition initiator (skA pkA pkB nA : val) : val := λ: <>,
   bind: "m1"   := aenc pkB (tuple nA pkA) in
   send "m1";;
   bind: "m2"   := adec skA (recv #()) in
   bind: "nA'"  := term_projV "m2" #0 in
   bind: "nB"   := term_projV "m2" #1 in
   bind: "pkB'" := term_projV "m2" #2 in
-  if: eq_term "pkB'" pkB then
+  if: eq_term "nA'" nA && eq_term "pkB'" pkB then
     bind: "m3" := aenc pkB "nB" in
     send "nB";;
     SOME "nB"
   else NONE.
 
-Definition responder (send recv skB pkB nB : val) : val := λ: <>,
+Definition responder (skB pkB nB : val) : val := λ: <>,
   bind: "m1"  := adec skB (recv #()) in
   bind: "nA" := term_projV "m1" #0 in
   bind: "pkA" := term_projV "m1" #1 in
@@ -91,5 +228,120 @@ Definition responder (send recv skB pkB nB : val) : val := λ: <>,
   send "m2";;
   bind: "nB'" := adec skB (recv #()) in
   if: "nB'" = nB then SOME "nA" else NONE.
+
+Hypothesis wp_send : forall E t,
+  ⊢ WP send t @ E {{v, ⌜v = #()⌝}}.
+
+Hypothesis wp_recv : forall E,
+  ⊢ WP recv #() @ E {{v, ∃ t, ⌜v = t⌝ ∗ termT RPub t}}.
+
+Ltac protocol_failure :=
+  by move=> *; iIntros "->"; wp_pures; iExists None.
+
+Lemma res_own l (r1 r2 : res Σ) :
+  own res_name (◯ {[l := to_agree r1]}) -∗
+  own res_name (◯ {[l := to_agree r2]}) -∗
+  r1 ≡ r2.
+Proof.
+iIntros "Hown1 Hown2".
+iPoseProof (own_valid_2 with "Hown1 Hown2") as "#Hvalid".
+rewrite auth_validI /= singleton_op gmap_validI.
+iSpecialize ("Hvalid" $! l).
+by rewrite lookup_singleton uPred.option_validI agree_validI agree_equivI.
+Qed.
+
+Lemma wp_initiator kA kB nA :
+  nsl_keys_inv -∗
+  nsl_sess_inv -∗
+  nonceT {[kA; kB]} nA -∗
+  initiator_key kA -∗
+  responder_key kB -∗
+  initiator_view (TNonce nA) SNew -∗
+  WP initiator (TKey KADec kA) (TKey KAEnc kA) (TKey KAEnc kB) (TNonce nA) #()
+     {{v, ∃ onB : option term,
+          ⌜v = repr onB⌝ ∗
+          match onB with
+          | Some nB => initiator_view (TNonce nA) (SAnswered nB true)
+          | None => True
+          end}}.
+Proof.
+rewrite /initiator.
+iIntros "Hkeys Hsess #HnA #HkA #HkB Hown".
+iPoseProof (initiator_key_akey with "Hkeys HkA") as "#HkA'".
+iPoseProof (responder_key_akey with "Hkeys HkB") as "#HkB'".
+wp_pures; wp_bind (tuple _ _).
+iApply twp_wp; iApply twp_wand; first by iApply twp_tuple.
+iIntros (?) "->".
+wp_bind (aenc _ _); iApply twp_wp; iApply twp_wand.
+  iApply twp_aenc; first by iExists ∅.
+  iLeft; iSplit; rewrite /=; last first.
+    iSplit.
+    - iExists {[kA; kB]}; iSplit; eauto.
+      iPureIntro; set_solver.
+    - iExists RPub, (agent_pred Init kA); iSplit; last by iPureIntro.
+      by iExists ∅.
+  by iModIntro; iSplit.
+iIntros (?) "[-> #Hm1]".
+wp_pures; wp_bind (send _); iApply wp_wand; first by iApply wp_send.
+iIntros (?) "->"; wp_pures.
+wp_bind (recv _); iApply wp_wand; first by iApply wp_recv.
+iIntros (?); iDestruct 1 as (m2) "[-> #Hm2]".
+wp_bind (adec _ _); iApply twp_wp; iApply twp_wand.
+  iApply twp_adec; eauto.
+iIntros (v).
+case: m2; try by protocol_failure.
+case; last by protocol_failure.
+move=> k t.
+case: decide; last by protocol_failure.
+move=> {k} ->; iDestruct 1 as "[-> #Ht]"; wp_pures.
+wp_bind (term_projV _ _).
+iApply twp_wp; iApply twp_wand; first by iApply (twp_term_projV _ _ 0).
+iIntros (?) "->".
+case enA': (term_proj t 0)=> [nA'|]; last by wp_pures; iExists None.
+wp_pures.
+wp_bind (term_projV _ _).
+iApply twp_wp; iApply twp_wand; first by iApply (twp_term_projV _ _ 1).
+iIntros (?) "->".
+case enB: (term_proj t 1)=> [nB|]; wp_pures; try by iExists None.
+wp_bind (term_projV _ _).
+iApply twp_wp; iApply twp_wand; first by iApply (twp_term_projV _ _ 2).
+iIntros (?) "->".
+case epkB': (term_proj t 2)=> [pkB'|]; wp_pures; try by iExists None.
+wp_bind (eq_term _ _).
+iApply twp_wp; iApply twp_wand; first by iApply twp_eq_term.
+iIntros (?) "->".
+case: bool_decide_reflect=> e; wp_pures; try by iExists None.
+subst nA'.
+wp_bind (eq_term _ _).
+iApply twp_wp; iApply twp_wand; first by iApply twp_eq_term.
+iIntros (?) "->".
+case: bool_decide_reflect=> e; wp_pures; try by iExists None.
+subst pkB'.
+iDestruct "Ht" as "[Ht|(_&Ht)]"; last first.
+  iPoseProof (term_proj_termT _ enA' with "Ht") as "contra".
+  iDestruct "contra" as (rs_nB) "[contra1 contra2]".
+  rewrite readers_subseteq_equiv.
+  case: rs_nB=> [|rs_nB]; last by iDestruct "contra2" as "[]".
+  iPoseProof (res_own with "HnA contra1") as "contra".
+  rewrite res_equivI.
+  by iPoseProof "contra" as "%contra".
+iDestruct "Ht" as "[#Hagent Ht]".
+case: t enA' enB epkB'=> // nA' [] // nB' [] // pkB' t' enA' enB epkB'.
+rewrite /= in enA' enB epkB'; move: enA' enB epkB'=> [->] [->] [->] {nA' nB' pkB'}.
+iSimpl in "Hagent".
+case: nB=> // nB.
+iDestruct "Hagent" as "(_&HnB&_&Hlb)".
+wp_bind (aenc _ _).
+iApply twp_wp; iApply twp_wand; first iApply twp_aencH.
+- iExists ∅. by iApply "HkB'".
+- iModIntro. iSimpl. iExists (TNonce nA), kA. iSplit; eauto.
+  iSplit; eauto. admit.
+- iExists {[kA; kB]}. iSplit=> //. iPureIntro. by set_solver.
+iIntros (?) "[-> #Hm3]".
+wp_pures.
+wp_bind (send _).
+iApply wp_wand; first iApply wp_send.
+iIntros (?) "->"; wp_pures; iExists (Some (TNonce nB)).
+Admitted.
 
 End NSL.
